\documentclass[oneside,12pt]{amsart}

\usepackage{amsmath,amssymb,latexsym,eucal,amsthm,graphicx}

\input{mathdefs}
\input{theoremstyles}

\graphicspath{{images/}}

\pagestyle{plain}

\begin{document}

\title{Solutions to Homework for Lesson 11 \\ Determinants}
\author{Math 325, Linear Algebra \\ Spring 2019\\ SFSU }
\date{}

\maketitle


\textbf{Problem 1} Exercise 1.9.1

\textbf{(a)}

\bigskip

$
\begin{pmatrix}
2 & -1 \\
-4 & 3
\end{pmatrix}
\SkipImplies
\begin{pmatrix}
2 & -1 \\
0 & 1
\end{pmatrix}
$

\bigskip

So the determinant is 2. Compare this to computing the determinant directly: 6-4=2.

\bigskip

\textbf{(b)}

\bigskip

$
\begin{pmatrix}
0 & 1 & -2 \\
-1 & 0 & 3 \\
2 & -3 & 0
\end{pmatrix}
\SkipImplies
\begin{pmatrix}
-1 & 0 & 3 \\
0 & 1 & -2 \\
2 & -3 & 0
\end{pmatrix}
\SkipImplies
\begin{pmatrix}
-1 & 0 & 3 \\
0 & 1 & -2 \\
0 & -3 & 6
\end{pmatrix}
\SkipImplies
\begin{pmatrix}
-1 & 0 & 3 \\
0 & 1 & -2 \\
0 & 0 & 0
\end{pmatrix}
$

\bigskip

So the determinant is 0, which coincides with the fact that the matrix is singular.

\textbf{(c)}

\bigskip

$
\begin{pmatrix}
1 & 2 & 3 \\
2 & 5 & 8 \\
3 & 8 & 10
\end{pmatrix}
\SkipImplies
\begin{pmatrix}
1 & 2 & 3 \\
0 & 1 & 2 \\
0 & 2 & 1
\end{pmatrix}
\SkipImplies
\begin{pmatrix}
1 & 2 & 3 \\
0 & 1 & 2 \\
0 & 0 & -3
\end{pmatrix}
$

\bigskip

So the determinant is -3.

\bigskip

\textbf{(d)}

\bigskip

$
\begin{pmatrix}
0 & 1 & -1 \\
-2 & 1 & 3 \\
2 & 7 & -8
\end{pmatrix}
\SkipImplies
\begin{pmatrix}
-2 & 1 & 3 \\
0 & 1 & -1 \\
2 & 7 & -8
\end{pmatrix}
\SkipImplies
\begin{pmatrix}
-2 & 1 & 3 \\
0 & 1 & -1 \\
0 & 8 & -5
\end{pmatrix}
\SkipImplies
\begin{pmatrix}
-2 & 1 & 3 \\
0 & 1 & -1 \\
0 & 0 & 3
\end{pmatrix}
$

\bigskip

The determinant of the row-echelon form matrix is -6. In doing Gaussian elimination
we performed one row-exchange. So the determinant of the original matrix is 6.

\bigskip

\textbf{(e)} This matrix is already in upper-triangular form. Its determinant
is the product of the entries on its main diagonal.

$5*3*-4*3 = -180$

\bigskip

You were not asked to do the rest of the parts but here are solutions
anyway.

\bigskip

\textbf{(f)}

\bigskip

$
\begin{pmatrix}
1 & -2 & 1 & 4 \\
2 & -4 & 0 & 0 \\
3 & -4 & 2 & 5 \\
0 & 2 & -4 & -9
\end{pmatrix}
\SkipImplies
\begin{pmatrix}
1 & -2 & 1 & 4 \\
0 & 0 & -2 & -8 \\
0 & 2 & -1 & -7 \\
0 & 2 & -4 & -9
\end{pmatrix}
\SkipImplies
\begin{pmatrix}
1 & -2 & 1 & 4 \\
0 & 2 & -1 & -7 \\
0 & 0 & -2 & -8 \\
0 & 2 & -4 & -9
\end{pmatrix}
\SkipImplies
\begin{pmatrix}
1 & -2 & 1 & 4 \\
0 & 2 & -1 & -7 \\
0 & 0 & -2 & -8 \\
0 & 0 & -3 & -2
\end{pmatrix}
\SkipImplies
\begin{pmatrix}
1 & -2 & 1 & 4 \\
0 & 2 & -1 & -7 \\
0 & 0 & -2 & -8 \\
0 & 0 & 0 & 10
\end{pmatrix}
$

The determinant of the upper-triangular matrix is the product of the
entries on its main diagonal: $1*2*-2*10=-40$. In doing Gaussian elimination
we performed one row-exchange. So the determinant of the original matrix is 40.


\bigskip

\textbf{(g)}

\bigskip

$
\begin{pmatrix}
1 & -2 & 1 & 4 & -5 \\
1 & 1 & -2 & 3 & -3 \\
2 & -1 & -1 & 2 & 2 \\
5 & -1 & 0 & 5 & 5 \\
2 & 2 & 0 & 4 & -1
\end{pmatrix}
\SkipImplies
\begin{pmatrix}
1 & -2 & 1 & 4 & -5 \\
0 & 3 & -3 & -1 & 2 \\
0 & 3 & -3 & -6 & 12 \\
0 & 9 & -5 & -15 & 30 \\
0 & 6 & -2 & -4 & 9
\end{pmatrix}
\SkipImplies
\begin{pmatrix}
1 & -2 & 1 & 4 & -5 \\
0 & 3 & -3 & -1 & 2 \\
0 & 0 & 0 & -5 & 10 \\
0 & 0 & 4 & -12 & 24 \\
0 & 0 & 4 & -2 & 5
\end{pmatrix}
\SkipImplies
\begin{pmatrix}
1 & -2 & 1 & 4 & -5 \\
0 & 3 & -3 & -1 & 2 \\
0 & 0 & 4 & -12 & 24 \\
0 & 0 & 0 & -5 & 10 \\
0 & 0 & 4 & -2 & 5
\end{pmatrix}
\SkipImplies
\begin{pmatrix}
1 & -2 & 1 & 4 & -5 \\
0 & 3 & -3 & -1 & 2 \\
0 & 0 & 4 & -12 & 24 \\
0 & 0 & 0 & -5 & 10 \\
0 & 0 & 0 & 10 & -19
\end{pmatrix}
\SkipImplies
\begin{pmatrix}
1 & -2 & 1 & 4 & -5 \\
0 & 3 & -3 & -1 & 2 \\
0 & 0 & 4 & -12 & 24 \\
0 & 0 & 0 & -5 & 10 \\
0 & 0 & 0 & 0 & 1
\end{pmatrix}
$

The determinant of the upper-triangular matrix is the product of the
entries on its main diagonal: $1*3*4*-5*1=-60$. In doing Gaussian elimination
we performed one row-exchange. So the determinant of the original matrix is 60.

\bigskip

\textbf{Problem 2} Exercise 1.9.3.

\bigskip

\textbf{(a)}

From part (b) we know that we need a matrix with determinant $\pm 1$.
And we are asked for a non-diagonal matrix. Let's just try the first
one that comes to mind:

Let
$$
A=
\begin{pmatrix}
0 & 1 \\
1 & 0
\end{pmatrix}
$$.

Trying it we see that $A^2=I$ so this is one solution.

\bigskip

\textbf{(b)} Suppose $A^2=I$. Then $1=\det(I) = \det(A^2) = \det(A)^2$.
There are only two real (or complex) numbers whose square is 1, so we
must have $\det(A) = \pm 1$.

\bigskip

\textbf{(c)} Let $x=\det(A)$ and suppose $A^2=A$. Then $x^2=x$ so $x^2-x=0$ so $x(x-1)=0$ so $x=0$ or $x=1$.

\bigskip

\textbf{Problem 3.} Exercise 1.9.4.

\bigskip

\textbf{(a)} If $\det(A)\not=0$ then $A^{-1}$ exists. Yes this is true.

\bigskip

\textbf{(b)} $\det(2A) = 2 \det A$. This is false. For example let $A$ be
the $2\times 2$ identity matrix. Then $\det(2A)=4$ but $2\det(A)=2$.

\bigskip

\textbf{(c)} $\det(A + B) = \det A + \det B$. This is false. This
follows from part (b) by letting $B=A$.

\bigskip

\textbf{(d)} $\det(A^{-\text{T}}) = \frac{1}{\det(A)}$. This is true because
$\det(A^{-\text{T}}) = \det\left( \transpose{A^{-1}} \right) = \det(A^{-1})$.

\bigskip

\textbf{(e)} $\det(AB^{-1}) = \frac{\det A}{\det B}$. This is true.

\bigskip

\textbf{(f)} $\det[(A + B)(A-B)] = \det( A^2 – B^2)$. This is false.
For example let
$A=
\begin{pmatrix}
1 & 0 \\
0 & 2
\end{pmatrix}
\text{ and }
B=
\begin{pmatrix}
0 & 1 \\
1 & 0
\end{pmatrix}
$

Then
$A+B=
\begin{pmatrix}
1 & 1 \\
1 & 2
\end{pmatrix}
\text{ and }
A-B=
\begin{pmatrix}
1 & -1 \\
-1 & 2
\end{pmatrix}
$

so

$\det[(A + B)(A-B)] = 1 \cdot 1 = 1$.

But

$A^2=
\begin{pmatrix}
1 & 0 \\
0 & 4
\end{pmatrix}
\text{ and }
B^2=
\begin{pmatrix}
1 & 0 \\
0 & 1
\end{pmatrix}
$

so

$
A^2 - B^2=
\begin{pmatrix}
0 & 0 \\
0 & 3
\end{pmatrix}
$

so

$\det( A^2 – B^2) = 0$.

\bigskip

\textbf{(g)} If $A$ is an $n \times n$ matrix with $\det A = 0$, then $\rank(A) < n$.

This is true. But we haven't learned about rank in class yet so you couldn't have answered this one.

\bigskip

\textbf{(h)} If $\det A = 1$ and $AB = O$, then $B = O$. This is true. In fact we
don't need $\det A = 1$, we only need $\det A \not= 0$. If $\det A \not= 0$ then
$A$ is invertible and multiplying both sides of the equation $AB = O$ on the left
by $A^{-1}$ we get that $B = O$.
\end{document}
