% $Header$

\documentclass{beamer}

\usepackage{amsmath,amssymb,latexsym,eucal,amsthm,graphicx}
\include{mathdefs}

\graphicspath{{images/}}

\newtheorem*{claim}{claim}
\newtheorem*{observation}{Observation}
\newtheorem*{warning}{Warning}
\newtheorem*{question}{Question}
\newtheorem{remark}[theorem]{Remark}

\newenvironment*{subproof}[1][Proof]
{\begin{proof}[#1]}{\renewcommand{\qedsymbol}{$\diamondsuit$} \end{proof}}

\mode<presentation>
{
  \usetheme{Singapore}
  % or ...

  \setbeamercovered{invisible}
  % or whatever (possibly just delete it)
}


\usepackage[english]{babel}
% or whatever

\usepackage[latin1]{inputenc}
% or whatever

\usepackage{times}
\usepackage[T1]{fontenc}
% Or whatever. Note that the encoding and the font should match. If T1
% does not look nice, try deleting the line with the fontenc.

\title{Lesson 5 \\ Linear functions $\R^n$}
\subtitle{Math 325, Linear Algebra \\ Fall 2018 \\ SFSU}
\author{Mitch Rudominer}
\date{}



% If you wish to uncover everything in a step-wise fashion, uncomment
% the following command:

\beamerdefaultoverlayspecification{<+->}

\begin{document}

\begin{frame}
  \titlepage
\end{frame}

\begin{frame}{Linear functions on $\R^n$}

\begin{itemize}
\item Let $f:\R^n \map \R^m$.
\item $f$ is called \emph{linear} iff $f$ satisfies the following two properties:
\item (i) For every two vectors $\bv, \bw \in\R^n$, $$f(\bv + \bw) = f(\bv) + f(\bw)$$
\item (ii) For all vectors $\bv\in\R^n$ and all scalars $c\in \R$,
$$f(c \bv) = c f(\bv)$$
\item In short we say ``f preserves vector addition and scalar multiplication.''
\end{itemize}

\end{frame}

\begin{frame}{$f$ Preserves Addition}

\begin{center}
\includegraphics[scale=0.25]{preserving-addition}
\end{center}

\begin{itemize}
\item $f(\bv + \bw) = f(\bv) + f(\bw)$
\item Let $f(\bv) = \bv^{\prime}$.
\item Let $f(\bw) = \bw^{\prime}$.
\item We can compute a vector sum on the left: $\bv + \bw$.
\item We can compute a vector sum on the right: $\bv^{\prime} + \bw^{\prime}$.
\item $f$ must move the vector sum on the left to the vector sum on the right.
\end{itemize}

\end{frame}

\begin{frame}{$f$ Preserves Scalar Multiplication}

\begin{center}
\includegraphics[scale=0.25]{preserving-scalar-mult}
\end{center}

\begin{itemize}
\item $f(c \bv) = c f(\bv)$
\item Let $f(\bv) = \bv^{\prime}$.
\item Let $c = 2$.
\item We can compute a scalar multiplication on the left: $2 \bv$.
\item We can compute a scalar multiplication on the right: $2 \bv^{\prime}$.
\item $f$ must move the scalar multiple on the left to the scalar multiple on the right.
\end{itemize}

\end{frame}

\begin{frame}{Example 1. $f:\R^1\map\R^1$}

\begin{itemize}
\item Let $f:\R^1\map\R^1$ be given by $f(x) = x^2$.
\item Is $f$ linear?
\item Check: Does $f$ preserve vector addition?
\item Note that on $\R^1$ vector addition is just ordinary addition of numbers.
\item $f(x_1 + x_2) = (x_1 + x_2)^2$
\item $= x_1^2 + x_2^2 + 2 x_1 x_2$
\item $= f(x_1) + f(x_2) + 2 x_1 x_2$.
\item So $f(x_1 + x_2) \not= f(x_1) + f(x_2)$
\item unless $2 x_1 x_2 = 0$, i.e. unless $x_1 = 0$ or $x_2 = 0$.
\item So $f$ is \emph{not} linear.
\end{itemize}

\end{frame}

\begin{frame}{Example 1. $f:\R^1\map\R^1$}

\begin{itemize}
\item Continue to let $f:\R^1\map\R^1$ be given by $f(x) = x^2$.
\item We already know $f$ is not linear.
\item Just for fun, check: Does $f$ preserve scalar multiplication?
\item $f(c x) = (c x)^2$
\item $= c^2 x^2$
\item $= c^2 f(x)$.
\item So $f(c x) \not= c f(x)$
\item unless $c^2 = c$, i.e. unless $c=0, 1$.
\item So again, $f$ is not linear.
\end{itemize}

\end{frame}

\begin{frame}{Example 2. $f:\R^1\map\R^1$}

\begin{itemize}
\item Let $f:\R^1\map\R^1$ be given by $f(x) = 2 x$.
\item Is $f$ linear?
\item Check: Does $f$ preserve vector addition?
\item $f(x_1 + x_2) =  2(x_1 + x_2)$
\item $ = 2 x_1 + 2 x_2$
\item $= f(x_1) + f(x_2)$.
\item So $f$ \emph{does} preserve addition.
\item Check: Does $f$ preserve scalar multiplication?
\item $f(c x) = 2 (c x)$
\item $ = c (2 x) $
\item $= c f(x)$.
\item So $f$ does preserve scalar multiplication.
\item So $f$ is linear.
\end{itemize}

\end{frame}

\begin{frame}{Example 3. $f:\R^3\map\R^2$}

\begin{itemize}
\item Consider this function from lesson 4:
\item $f(x,y,z) = (x, x^2)^{\text{T}}$
\item Is $f$ linear?
\item Check: Does $f$ preserve vector addition?
\item Let $\bv, \bw \in \R^2$
\item We need to check if $f(\bv + \bw) = f(\bv) + f(\bw)$
\end{itemize}

\end{frame}

\beamerdefaultoverlayspecification{}

\begin{frame}{Does $f$ preserve vector addtion?}
\begin{align*}
&f(\bv + \bw) \\
\uncover<2->{&=  f\bigl((v_1, v_2,v_3)^{\text{T}} + (w_1, w_2,w_3)^{\text{T}} \bigr) \\}
\uncover<3->{&= f(v_1 + w_1, v_2 + w_2, v_3+w_3) \\}
\uncover<4->{&= \left(v_1 + w_1, (v_1 + w_1)^2  \right)^{\text{T}}  \\}
\uncover<5->{&= \left(v_1 + w_1, v_1^2 + w_1^2 + 2v_1 w_1  \right)^{\text{T}} \\}
\uncover<6->{&= \left(v_1, v_1^2 \right)^{\text{T}} + \left(w_1, w_1^2 \right)^{\text{T}} + \left(0, 2v_1 w_1  \right)^{\text{T}} \\}
\uncover<7->{&= f(v_1, v_2,v_3) + f(w_1, w_2,w_3)  + \left(0, 2v_1 w_1  \right)^{\text{T}} \\}
\uncover<8->{&= f(\bv) + f(\bw)  + \left(0, 2v_1 w_1  \right)^{\text{T}} \\}
\uncover<9->{&\not= f(\bv) + f(\bw) \text{ unless $v_1=0$ or $w_1=0$}\\}
\end{align*}
\uncover<10->{So $f$ does not preserve vector addtion. So $f$ is not linear.}
\end{frame}

\beamerdefaultoverlayspecification{<+->}

\begin{frame}{Linear Functionals}

\begin{itemize}
\item A linear function from $\R^n$ to $\R^1$ is also called a linear
\emph{functional}.
\item Let $\bv \in \R^n$ be any vector.
\item We will show how $\bv$ can used as a linear functional.
\item In its role as a linear functional, $\bv$ is called a \emph{covector}.
\item Let $f_{\bv} : \R^n \map \R^1$ be defined by
$$f_{\bv}(\bw) = \bv \cdot \bw$$
\item $f_{\bv}$ is called the \emph{covector} associated to the vector $\bv$.
\end{itemize}

\end{frame}

\begin{frame}{Example Covector}

\begin{itemize}
\item Let $\bv = (2, -1)$
\item So $f_{\bv}:\R^2 \map \R$.
\item Let $\bw = (4, 5) \in \R^2$.
\item Compute $f_{\bv}(\bw)$
\item $= \bv \cdot \bw = 8 - 5 = 3$
\item $f_{\bv}(\bw) =  3$.
\end{itemize}

\end{frame}

\begin{frame}{Dot Product is Linear}

\begin{itemize}
\item Claim: For any vector $\bv\in\R^n$, $f_{\bv}:\R^n\map\R$ is linear.
\item proof:
\item First we show that $f_{\bv}$ preserves vector addition.
\item Let $\bu, \bw \in \R^n$
\item We must show $f_{\bv}(\bu + \bw) = f_{\bv}(\bu) + f_{\bv}(\bw)$
\item i.e. that $\bv \cdot (\bu + \bw) = \bv \cdot \bu + \bv \cdot \bw$.
\item This is just the distributive law for dot product.
\end{itemize}

\end{frame}

\beamerdefaultoverlayspecification{}

\begin{frame}{Distributive law for dot product}
\begin{align*}
f_{\bv}(\bu + \bw)
\uncover<2->{&= \bv \cdot (\bu + \bw) }\\
\uncover<3->{&=  \sum_i{v_i (u_i + w_i)} \\}
\uncover<4->{&= \sum_i{v_i u_i +v_i  w_i} \\}
\uncover<5->{&= \sum_i{v_i u_i} + \sum_i{v_i  w_i} \\}
\uncover<6->{&= \bv \cdot \bu + \bv \cdot \bw \\}
\uncover<7->{&= f_{\bv}(\bu) + f_{\bv}(\cdot \bw)}
\end{align*}

\end{frame}

\beamerdefaultoverlayspecification{<+->}

\begin{frame}{Dot Product is Linear (2)}

\begin{itemize}
\item So $f_{\bv}$ preserves vector addition.
\item Now we must show that $f_{\bv}$ preserves scalar multiplication.
\item Let $\bu \in \R^n$ and let $c\in\R$.
\item We must show $f_{\bv}(c \bu) = c f_{\bv}(\bu)$
\item i.e. that $\bv \cdot (c \bu) = c (\bv \cdot \bu)$
\end{itemize}

\end{frame}

\beamerdefaultoverlayspecification{}

\begin{frame}{Dot Product is Linear (3)}
\begin{align*}
f_{\bv}(c \bu)
\uncover<2->{&= \bv \cdot (c \bu) }\\
\uncover<3->{&=  \sum_i{v_i (c u_i)} \\}
\uncover<4->{&= c \sum_i{v_i u_i } \\}
\uncover<5->{&= c (\bv \cdot \bu) \\}
\uncover<6->{&= c f_{\bv}(\bu)}
\end{align*}

\end{frame}

\beamerdefaultoverlayspecification{<+->}

\begin{frame}{Dot Product is Linear (4)}

\begin{itemize}
\item So $f_{\bv}$ preserves scalar multiplication.
\item So $f_{\bv}$ is linear. $\qed$.
\end{itemize}

\end{frame}

\begin{frame}{Linear functions preserve linear combinations}
\begin{lemma}
Let $f:\R^n\map\R^m$. The following are equivalent:
\begin{enumerate}
\item $f$ is linear
\item $f$ preserves all linear combinations.

\pause

i.e. for every
$\bw_1,\bw_2,\cdots\bw_k\in\R^n$, for every $c_1,c_2,\cdots c_k\in\R$,
$$f(c_1 \bw_1 + c_2 \bw_2 + \cdots + c_k \bw_k) = c_1 f(\bw_1) + c_2 f(\bw_2) + \cdots + c_k f(\bw_k)$$

\pause

\item $f$ preserves linear combinations of length 2.

\pause

i.e. for every $\bw_1,\bw_2\in\R^n$, for every $c_1,c_2\in\R$,
$f(c_1 \bw_1 + c_2 \bw_2) = c_1 f(\bw_1) + c_2 f(\bw_2) f(\bw_k)$.

\end{enumerate}
\end{lemma}
\end{frame}


\begin{frame}{Example: Covector preserves linear combinations}

\begin{itemize}
\item Let $\bv = (2, -1)$
\item So $f_{\bv}:\R^2 \map \R$.
\item Let $\bw_1 = (4, 5) \in \R^2$.
\item Let $\bw_2 = (1,-1) \in \R^2$.
\item $f_\bv(2\bw_1 -3\bw_2)$
\item $=f_\bv\bigl((5, 13)\bigr)$
\item $=\bv \cdot (5, 13)$
\item $=10 - 13 = -3$.
\item $2 f_{\bv}(\bw_1) -3 f_{\bv}(\bw_2)$
\item $= 2 (\bv \cdot \bw_1) -3 (\bv \cdot \bw_2)$
\item $=2 (3) - 3(3)$
\item $=-3$
\item So $f_\bv(2\bw_1 -3\bw_2) = 2f_{\bv}(\bw_1) -3 f_{\bv}(\bw_2)$.
\end{itemize}

\end{frame}

\begin{frame}{Proof of Lemma}

\begin{itemize}
\item (3) $\implies$ (1). Suppose that $f$ preserves linear combinations of length 2.
\item $f(c_1 \bw_1 + c_2 \bw_2) = c_1 f(\bw_1) + c_2 f(\bw_2)$.
\item Letting $c2=0$ we have
\item $f(c_1 \bw_1) = c_1 f(\bw_1)$.
\item So $f$ preserves scalar multiplication.
\item Letting $c_1 = c_2 = 1$ we have
\item $f(\bw_1 + \bw_2) = f(\bw_1) + f(\bw_2)$.
\item So $f$ preserves vector addition.
\item So $f$ is linear.
\item (2) $\implies$ (3) is trivial. So we are left with...
\item (1) $\implies$ (2). Suppose $f$ is linear.
\item We must show that $f$ preserves all linear combinations.
\item This is done by induction on $k$.
\item The base case, $k=1$, says $f(c_1 \bw_1) = c_1 f(\bw_1)$.
\item This follows from the fact that $f$ preserves scalar mult.
\end{itemize}

\end{frame}

\beamerdefaultoverlayspecification{}

\begin{frame}{The inductive step}
Now suppose that
$$f\left(\Sigma_{i=1}^k{c_i \bw_i}\right) = \Sigma_{i=1}^k{c_i f(\bw_i)}$$

\smallskip

We must show that
$$f\left(\Sigma_{i=1}^{k+1}{c_i \bw_i}\right) = \Sigma_{i=1}^{k+1}{c_i f(\bw_i)}$$

\begin{align*}
&f\left(\Sigma_{i=1}^{k+1}{c_i \bw_i}\right)\\
\uncover<2->{&=  f\left(\Sigma_{i=1}^{k}{c_i \bw_i} + c_{k+1} \bw_{k+1}\right)\\}
\uncover<3->{&=  f\left(\Sigma_{i=1}^{k}{c_i \bw_i}\right) + f(c_{k+1} \bw_{k+1}) \quad \text{ ($f$ preserves addition)} \\}
\uncover<4->{&= \Sigma_{i=1}^k{c_i f(\bw_i)} + f(c_{k+1} \bw_{k+1}) \quad \text{ (induction)}\\}
\uncover<5->{&= \Sigma_{i=1}^k{c_i f(\bw_i)} + c_{k+1} f(\bw_{k+1}) \quad \text{ ($f$ preserves scalar mult.)}\\}
\uncover<6->{&= \Sigma_{i=1}^{k+1}{c_i f(\bw_i)} }
\end{align*}

\uncover<7->{So $f$ preserves all linear combinations. $\qed$.}
\end{frame}

\beamerdefaultoverlayspecification{<+->}

\begin{frame}{Arbitrary functions are flexible}
\begin{itemize}
\item Suppose $f:\R^2\map\R$ is \emph{some} function. (Not necessarily linear).
\item Suppose I told you that $f(0,1) = 12$
\item and I told you that $f(1, 0) = -1$.
\item Question: What is $f(2, 2)$?
\item Answer: You have no idea. It could be anything.
\item Arbitrary functions are "flexible". They can bend however you want them to.
\item Knowing the value of $f$ at any finite number of points tells you nothing
about the value of $f$ at any other point.
\item Now suppose I told you $f$ were linear?
\item Then $f(2,2) = f\left(2(1,0) + 2(0,1)\right)$
\item $=2f(1,0) + 2f(0,1)$
\item $= 2(12) + 2 (-1) = 23$.
\end{itemize}
\end{frame}

\beamerdefaultoverlayspecification{}

\begin{frame}{Values at the standard basis vectors}

A linear function is determined by its values at the standard basis vectors.

\uncover<2->{
\begin{lemma}
Let $f:\R^n\map\R^m$ and $g:\R^n\map\R^m$  be two linear functions. \\
\uncover<3->{Suppose that $f(\be_i) = g(\be_i)$ for $i=1, 2, \cdots n$.} \\
\uncover<4->{Then $f = g$.}
\end{lemma}
}

\end{frame}

\begin{frame}{Proof of Lemma}

\begin{proof}
Assume $f(\be_i) = g(\be_i)$ for $i=1, 2, \cdots n$.
Let $\bv\in\R^n$ be any vector.
\uncover<2->{We must show that $f(\bv)=g(\bv)$.}
\uncover<3->{
Now $\bv = (v_1,v_2,\cdots v_n)$.
So $\bv=\sum_i{v_i \be_i}$.
}

\begin{align*}
\uncover<4->{f(\bv) &= f\left(\sum_i{v_i \be_i}\right) \\}
\uncover<5->{&= \sum_i{v_i f(\be_i)} \text{ \qquad (by linearity)}\\}
\uncover<6->{&= \sum_i{v_i g(\be_i)} \text { \qquad (by assumption)}\\}
\uncover<7->{&= g\left(\sum_i{v_i \be_i}\right) { \qquad  (by linearity)} \\}
\uncover<8->{&= g(\bv)}
\end{align*}
\end{proof}
\end{frame}

\beamerdefaultoverlayspecification{<+->}

\begin{frame}{All functionals are covectors}

All functionals on $\R^n$ are given by covectors.

\pause

\begin{lemma}
Let $f:\R^n\map\R$ be a covector.\\
\pause
Then there is a vector $\bv\in\R^n$ such that $f=f_{\bv}$. \\
\end{lemma}

\pause

\begin{itemize}
\item Proof:
\item Let $a_i = f(\be_i)$ for $i=1,\cdots n$.
\item Let $\bv=(a_1, a_2, \cdots a_n)$.
\item Notice $\bv\cdot\be_i=a_i$ for $i=1,\cdots n$.
\item So $f_{\bv}(\be_i)=a_i$ for $i=1,\cdots n$.
\item So $f_{\bv}(\be_i)=f(\be_i)$ for $i=1,\cdots n$.
\item By the previous lemma, $f = f_{\bv}$. $\qed$
\end{itemize}

\end{frame}

\begin{frame}{Linear component functions}

A function is linear iff it's component functions are.

\pause

\begin{lemma}
Let $f:\R^n\map\R^m$ be a function.\\
\pause
Write $f(\bv) = \left(f_1(\bv),f_2(\bv),\cdots f_m(\bv)\right)$. \\
\pause
Then the following are equivalent:
\pause
\begin{enumerate}
\item $f$ is linear
\item $f_i$ is linear for $i=1,\dots m$.
\end{enumerate}
\end{lemma}

\pause

\begin{itemize}
\item Proof:
\item Let $\bv_1,\dots\bv_n\in\R^n$ and let $c_1,\dots c_n \in\R$.
\item $f\left(\sum_j{c_j \bv_j}\right) = \sum_j{c_j f(\bv_j)}$
\item iff $\left(f_1\left(\sum_j{c_j \bv_j}\right),\cdots,f_m\left(\sum_j{c_j \bv_j}\right)\right) = \left( \sum_j{c_j f_1(\bv_j)},\cdots \sum_j{c_j f_m(\bv_j)} \right)$
\item iff $f_i\left(\sum_j{c_j \bv_j}\right) = \sum_j{c_j f_i(\bv_j)}$, for $i=1,\dots m$.
\end{itemize}

\end{frame}

\begin{frame}{Characterization of linear functions}

All linear functions from $\R^n$ to $\R^m$ are given by $m$ covectors.

\pause

\begin{theorem}
Let $f:\R^n\map\R^m$ be a linear function.\\
\pause
Then there are $m$ vectors $\bv_1,\bv_2,\cdots\bv_m \in \R^n$ such that
$f = \left(f_{\bv_1}, f_{\bv_2}, \cdots f_{\bv_m}\right)$.

\pause
\smallskip

Conversely, Let $\bv_1,\bv_2,\cdots\bv_m$ be any $m$ vectors in $\R^n$ and
let $f=\left(f_{\bv_1}, f_{\bv_2},\cdots f_{\bv_n}\right)$.
\pause
Then $f:\R^n\map\R^m$ is linear.

\end{theorem}

\end{frame}

\begin{frame}{Proof of theorem}

\begin{itemize}
\item Let $f:\R^n\map\R^m$ be a linear function.
\item Write $f = (f_1, f_2, \cdots f_m)$.
\item From a previous lemma each $f_i$ is linear.
\item But $f_i:\R^n\map\R$ so each $f_i$ is a linear functional.
\item But all linear functionals are covectors.
\item So for each $i$, let $\bv_i$ be such that $f_i = f_{\bv_i}$.
\item Then $f=(f_{\bv_1}, f_{\bv_2},\cdots f_{\bv_n})$.
\item Conversely, let $\bv_1,\bv_2,\cdots\bv_m$ be any $m$ vectors in $\R^n$.
\item Let $f=(f_{\bv_1}, f_{\bv_2},\cdots f_{\bv_n})$.
\item Since each of the component functions of $f$ is linear, $f$ is linear.
\end{itemize}


\end{frame}

\begin{frame}{Example: A linear $f:\R^2\map\R^3$}
According to the theorem, a linear function from $\R^2$ to $\R^3$ is
given by three covectors from $\R^2$.

\begin{itemize}
\item Let $\bv_1 = (2, 1)$
\item Let $\bv_2 = (0, -3)$
\item Let $\bv_3 = (-1, 0)$
\item Let $f = (f_{\bv_1},f_{\bv_2},f_{\bv_3})$.
\item Then $f:\R^2\map\R^3$ is linear.
\item Let $\bw = (3, -2)$. Compute $f(\bw)$.
\item $f(\bw) = \left(f_{\bv_1}(\bw),f_{\bv_2}(\bw),f_{\bv_3}(\bw)\right)$
\item $=(4, 6, -3)$
\end{itemize}

\end{frame}

\begin{frame}{Linear functions given by values at the standard basis vectors.}

There exists a unique linear function with any specified values for the
standard basis vectors.

\pause

\begin{theorem}
Let $\bw_1,\bw_2,\cdots\bw_n \in \R^m$. Then there exists a unique linear
function $f:\R^n\map\R^m$ such that
$$f(\be_i) = \bw_i, \text{ for } 1\leq i \leq n$$
\end{theorem}

\pause

Proof:

\begin{itemize}
\item An earlier lemma already gave us uniqueness.
(Linear functions are determined by their values on the standard basis vectors.)
So we only have to prove existence.
\item Let $\bv\in\R^n$. We have to define $f(\bv)$.
\item Now $\bv = \sum_i{v_i \be_i}$.
\end{itemize}

\end{frame}

\begin{frame}{Proof continued}

\begin{itemize}
\item If $f$ is going to be linear we have no choice but to define
\item $f(\bv) = \sum_i{v_i  f(\be_i)}$
\item $=\sum_i{v_i  \bw_i}$.
\item This is linear:
\item $f(c_1 \bu + c_2\bv)$
\item $=f(\sum_i{(c_1\cdot u_i +c_2 \cdot v_i)\be_i})$
\item $= \sum_i{(c_1\cdot u_i +c_2 \cdot v_i)\bw_i}$ \quad (definition of $f$)
\item $= c_1\sum_i{u_i \bw_i} +c_2\sum_i{v_i \bw_i}$
\item $= c_1f(\bu) +c_2 f(\bv)$ \quad (definition of $f$).
\end{itemize}

\pause

So $f$ is linear. $\qed$.

\end{frame}

\begin{frame}{Example: A linear $f:\R^2\map\R^3$}
According to the theorem, a linear function from $\R^2$ to $\R^3$ is
given by two vectors in $\R^3$ to be the images of the two standard
basis vectors in $\R^2$.

\begin{itemize}
\item Let $\bw_1 = (2, 0, -1)$.
\item Let $\bw_2 = (1, -3, 0)$.
\item According to the theorem there is a unique linear $f:\R^2\map\R^3$ such that
\item $f(\be_1) = \bw_1$ and $f(\be_2) = \bw_2$.
\item Let $\bu = (3, -2)$. Compute $f(\bw)$.
\item $f(\bu) = f(3\be_1 -2\be_2)$
\item $=3 \bw_1 -2\bw_2$
\item $=(4, 6, -3)$
\end{itemize}

\end{frame}

\begin{frame}{Two ways of specifying linear $f:\R^n\map\R^m$}

\begin{itemize}
\item We now have two ways of specifiying a linear function $f:\R^n\map\R^m$:
\item By giving $m$ covectors from $\R^n$.
\item By giving $n$ vectors in $\R^m$.
\item Notice that in our two examples we got the same result for $f(3,-2)$.
\item Actually we specified the same linear function both times, but in
the two different ways.
\item This fact will become more clear when we switch to expressing these
ideas using matrices in the next lesson.
\end{itemize}

\end{frame}


\begin{frame}{Composition of linear functions}

The composition of linear functions is linear.

\pause

\begin{lemma}
Let $f:\R^n\map\R^m$ be linear. Let $g:\R^m\map\R^k$ be linear.
Let $h:\R^n\map\R^k$ be given by $h=g\circ f$.
\pause
Then $h$ is linear.
\end{lemma}

\pause

proof:

\begin{itemize}
\item $h(a\bv +b\bw)$
\item $= g(f(a\bv +b\bw))$
\item $= g(a f(\bv) + b f(\bw))$ \quad (because $f$ is linear)
\item $= a g(f(\bv)) + b g(f(\bw))$ \quad (because $g$ is linear)
\item $= a h(\bv) + b h(\bw)$.
\item So $h$ is linear. $\qed$.
\end{itemize}

\end{frame}

\begin{frame}{Example Composition}

Let $f:\R^2\map\R^3$ be the function we considered a few slides back:

\begin{itemize}
\item Let $\bv_1 = (2, 1)$
\item Let $\bv_2 = (0, -3)$
\item Let $\bv_3 = (-1, 0)$
\item Let $f = (f_{\bv_1},f_{\bv_2},f_{\bv_3})$.
\item So $f:\R^2\map\R^3$ is linear.
\item Now let $\bu\in\R^3 = (-1, -1, 2)$.
\item Then $g = f_{\bu}:\R^3\map\R$ is a covector from $\R^3$.
\item Now let $h=g\circ f$.
\item Then $h:\R^2\map\R^1$. According to the theorem it is linear.
\item Let $\bw = (3, -2)$. Compute $h(\bw)$.
\item From our earlier example $f(\bw) =(4, 6, -3)$.
\item So $h(\bw) = g(4, 6, 3)$ = $\bu\cdot(4,6,3) = -4 -6 -6 = -16$.
\end{itemize}

\end{frame}

\begin{frame}{Operations on linear functions}

We can consider the \emph{set of all} linear functions from $\R^n$ to $\R^m$.

\begin{itemize}
\item Let $L(\R^n,\R^m)$ mean the set of all linear functions from $\R^n$ to $\R^m$.
\item There are a few \emph{operations} that make sense on $L(\R^n, \R^m)$.
\item Addition:
\item Let $f, g \in L(\R^n, \R^m)$. We can define $f+g$.
\item Scalar multiplication:
\item Let $f\in L(\R^n, \R^m)$. Let $c\in\R$. We can define $cf$.
\end{itemize}

\end{frame}

\begin{frame}{Addition of linear functions}

\begin{itemize}
\item Let $f, g \in L(\R^n,\R^m)$.
\item We want to define $h = f+g \in L(\R^n,\R^m)$.
\item Now $f:\R^n\map\R^m$ and $g:\R^n\map\R^m$.
\item We want to define $h:\R^n\map\R^m$.
\item How should we define $h$?
\item Let $\bv\in\R^n$. What should $h(\bv)$ be?
\item $h(\bv) = (f+g)(\bv) = ?$
\item $=f(\bv) + g(\bv)$.
\end{itemize}

\end{frame}

\begin{frame}{Sum of linear functions is linear}

\begin{lemma}
Let $f,g\in L(\R^n, \R^m)$. Then $f+g$ is linear.
\end{lemma}

\pause

Proof:

\pause

\begin{itemize}
\item $(f+g)(c_1 \bv_1 + c_2 \bv_2)$
\item $=f(c_1 \bv_1 + c_2 \bv_2) + g(c_1 \bv_1 + c_2 \bv_2)$ \quad (Definition of $f+g$)
\item $=c_1f(\bv_1)+ c_2f(\bv_2) + c_1g(bv_1) + c_2g(\bv_2)$ \quad ($f$ and $g$ are both linear)
\item $= c_1\left(f(\bv_1)+  g(bv_1)\right) + c_2\left(f(\bv_2) + g(\bv_2)\right)$
\item $=c_1\left((f + g)(\bv_1)\right) + c_2\left((f+g)(\bv_2) \right)$ \quad (Definition of $f+g$)
\end{itemize}

\pause

So $f+g$ is linear. $\qed$.

\end{frame}

\begin{frame}{Scalar multiplication of linear functions}

\begin{itemize}
\item Let $f \in L(\R^n,\R^m)$. Let $c\in\R$.
\item We want to define $h = c f \in L(\R^n,\R^m)$.
\item Now $f:\R^n\map\R^m$.
\item We want to define $h:\R^n\map\R^m$.
\item How should we define $h$?
\item Let $\bv\in\R^n$. What should $h(\bv)$ be?
\item $h(\bv) = (c f)(\bv) = ?$
\item $= c \left(f (\bv)\right)$.
\end{itemize}

\end{frame}

\begin{frame}{Scalar multiple of a linear function is linear}

\begin{lemma}
Let $f\in L(\R^n, \R^m)$. Let $c\in\R$. Then $c f$ is linear.
\end{lemma}

\pause

Proof:

\pause

\begin{itemize}
\item $(c f)(c_1 \bv_1 + c_2 \bv_2)$
\item $=c \left (f(c_1 \bv_1 + c_2 \bv_2) \right )$ \quad (Definition of $c f$)
\item $= c \left(c_1 f(\bv_1) + c_2 f(\bv_2)  \right)$ \quad ($f$ is linear)
\item $= \left(c_1 \cdot c \cdot f(\bv_1) + c_2 \cdot c \cdot f(\bv_2)  \right)$
\item $= \left(c_1 (c f)(\bv_1) + c_2 (c f)(\bv_2)  \right)$ \quad (Definition of $c f$)
\end{itemize}

\pause

So $c f$ is linear. $\qed$.

\end{frame}

\end{document}


