% $Header$

%\documentclass{beamer}
\documentclass[handout]{beamer}
\usepackage{amsmath,amssymb,latexsym,eucal,amsthm,graphicx,hyperref}
\input{mathdefs}

\graphicspath{{images/}}

\newtheorem*{claim}{claim}
\newtheorem*{observation}{Observation}
\newtheorem*{warning}{Warning}
\newtheorem*{question}{Question}
\newtheorem{remark}[theorem]{Remark}

\newenvironment*{subproof}[1][Proof]
{\begin{proof}[#1]}{\renewcommand{\qedsymbol}{$\diamondsuit$} \end{proof}}

\mode<presentation>
{
  \usetheme{Singapore}
  % or ...

  \setbeamercovered{invisible}
  % or whatever (possibly just delete it)
}


\usepackage[english]{babel}
% or whatever

\usepackage[latin1]{inputenc}
% or whatever

\usepackage{times}
\usepackage[T1]{fontenc}
% Or whatever. Note that the encoding and the font should match. If T1
% does not look nice, try deleting the line with the fontenc.

\title{Lesson 12 \\ Modular Arithmetic}
\subtitle{Math 310, Elementary Number Theory \\ Fall 2020 \\ SFSU}
\author{Mitch Rudominer}
\date{}



% If you wish to uncover everything in a step-wise fashion, uncomment
% the following command:

\beamerdefaultoverlayspecification{<+->}

\begin{document}

\begin{frame}
  \titlepage
\end{frame}

\begin{frame}{Doing the same thing to both sides}

\begin{itemize}
  \item We can do some simple algebra with congruences.
  \item Suppose $x,y,c,m$ are integers with $m>1$.
  \item Suppose $x\equiv y \pmod m$.
  \item Then you can conclude that:
  \item $x+c\equiv y+c \pmod m$
  \item $x-c\equiv y-c \pmod m$
  \item $cx \equiv cy \pmod m$.
  \item For example, suppose $x\equiv y \pmod {37}$.
  \item Then $x+111\equiv y+111 \pmod {37}$.
  \item $7x \equiv 7y \pmod {37}$.
\end{itemize}

\end{frame}

\begin{frame}{Justification}

\begin{itemize}
  \item Why is this simple algebra justified?
  \item Suppose $x\equiv y \pmod m$.
  \item So $m \divides (x-y)$.
  \item So $m \divides \big( (x+c) - (y+c) \big)$.
  \item And $m \divides (cx - cy)$.
\end{itemize}

\end{frame}

\begin{frame}{Example}

\begin{itemize}
  \item True or false: $7,953 \equiv  4,953 \pmod 3$?
  \item $7\equiv 4  \pmod 3$.
  \item So $7000 \equiv 4000 \pmod 3$.
  \item $7,953 \equiv  4,953 \pmod 3$.
\end{itemize}

\end{frame}

\begin{frame}{What about cancellation?}

\begin{itemize}
  \item True or false:
  \item If $cx \equiv cy \pmod m$ then $x\equiv y \pmod m$.
  \item Example: $20 \equiv 35 \pmod {15}$.
  \item $5\cdot 4 \equiv 5 \cdot 7 \pmod {15}$
  \item Does it follow that $4 \equiv 7 \pmod {15}$?
  \item No.
\end{itemize}

\end{frame}

\begin{frame}{Cancellation when $c$ and $m$ are relatively prime.}
\begin{itemize}
  \item \textbf{Lemma.} Suppose $x,y,c,m$ are integers with $m>1$.
  \item Suppose that $\gcd(c, m) = 1$.
  \item Suppose that $cx \equiv cy \pmod m$.
  \item Then $x\equiv y \pmod m$.
  \item Example: $35 \equiv 50 \pmod 3$.
  \item $5\cdot 7 \equiv 5 \cdot 10 \pmod 3$.
  \item Because $\gcd(5,3) = 1$ we can cancel the 5.
  \item Conclude: $7\equiv 10 \pmod 3$.
\end{itemize}
\end{frame}

\begin{frame}{Proof}
\begin{itemize}
  \item Suppose that $cx \equiv cy \pmod m$.
  \item So $m \divides c(x-y)$.
  \item In general we cannot conclude that $m \divides (x-y)$.
  \item But, if $\gcd(m,c) = 1$ then we can conclude that $m\divides (x-y)$.
  \item So $x\equiv y \pmod m$.
\end{itemize}
\end{frame}

\begin{frame}{Factoring the modulus}
\begin{itemize}
  \item Suppose that $x\equiv y \pmod {cm}$.
  \item Then $x\equiv y \pmod m$.
  \item Example: If $x\equiv y \pmod 9$,
  \item Then $x\equiv y \pmod 3$.
  \item Saying that $x\equiv y \pmod 9$ is \emph{stronger} than saying that $x\equiv y \pmod 3$.
  \item Proof: If $cm \divides (x-y)$ then $m\divides (x-y)$.
\end{itemize}
\end{frame}

\begin{frame}{Cancellation and Factoring the modulus}
\begin{itemize}
  \item Example: $28 \equiv 48 \pmod {10}$.
  \item $4\cdot 7 \equiv 4 \cdot 12 \pmod {10}$
  \item It does \emph{not} follow that $7 \equiv 12 \pmod {10}$
  \item But:  $4\cdot 7 \equiv 4 \cdot 12 \pmod {2\cdot 5}$
  \item Then:  $4\cdot 7 \equiv 4 \cdot 12 \pmod {5}$, and $\gcd(4,5) = 1$
  \item So:  $7 \equiv  12 \pmod {5}$
  \item \textbf{Lemma.} Suppose $x,y,c,m$ are integers with $m>1$.
  \item Let $d=\gcd(c,m)$.
  \item If $cx\equiv cy \pmod m$.
  \item Then $x\equiv y \pmod {m/d}$.
\end{itemize}
\end{frame}

\begin{frame}{Example}
\begin{itemize}
  \item Example: $12 \equiv 30 \pmod {9}$.
  \item $6 \cdot 2 \equiv 6 \cdot 5 \pmod {9}$.
  \item We cannot conclude that $2\equiv 5 \pmod {9}$.
  \item But $\gcd(6,9) = 3$.
  \item We can conclude that $2\equiv 5 \pmod {9/3}$.
  \item $2\equiv 5 \pmod 3$.
\end{itemize}
\end{frame}

\begin{frame}{Example}
\begin{itemize}
  \item Example: $18 \equiv 30 \pmod {12}$.
  \item $6 \cdot 3 \equiv 6 \cdot 5 \pmod {6\cdot 2}$.
  \item We cannot conclude that $3\equiv 5 \pmod {12}$.
  \item But we can conclude that $3\equiv 5 \pmod 2$.
\end{itemize}
\end{frame}

\begin{frame}{Modular addition and multiplication}
\begin{itemize}
  \item \textbf{Lemma.} Suppose $a \equiv \aprime \pmod {m}$.
  \item and $b  \equiv \bprime \pmod {m}$.
  \item Then $a+b \equiv \aprime + \bprime \pmod {m}$
  \item and $a \cdot b \equiv \aprime \cdot \bprime \pmod {m}$.
  \item Example: $6 \equiv 11 \pmod 5$ and $13\equiv 23 \pmod 5$.
  \item So $(6+13) \equiv (11 +23) \pmod 5$
  \item and  $6\cdot 13 \equiv 11\cdot 23 \pmod 5$.
  \item Interpretation using ``slots and blocks'':
  \item If you only want to know the slot
  of the result you only need to know the slots of the arguments.
\end{itemize}
\end{frame}

\begin{frame}{Proof}
\begin{itemize}
  \item We have already seen something equivalent to this lemma.
  \item Recall that $(a+b)\bmod m = \big( (a\bmod m) + (b\bmod m) \big) \bmod m$,
  \item and $(a\cdot b)\bmod m = \big( (a\bmod m) \cdot (b\bmod m) \big) \bmod m$.
  \item But this means that to compute the sum or product mod $m$, the only thing that
  matters about $a$ and $b$ are their values mod $m$.
  \item So $a$ can be replaced by
  $\aprime$ and $b$ can be replaced by $\bprime$ without changing the value of
  the sum or product mod $m$.
\end{itemize}
\end{frame}

\begin{frame}{Example}
\begin{itemize}
  \item Compute $(1! + 2! + 3! + \cdots + 100!) \pmod 9$.
  \item Solution: Notice that $9\divides n!$ for $n\geq 6$.
  \item So we can reduce to $(1! + 2! + 3! + 4! + 5!) \pmod 9$.
  \item $2! \bmod 9 = 2$
  \item $3! \bmod 9 = 6$
  \item $4! \bmod 9 = 24 \bmod 9 = 6$.
  \item $5! = 5 \cdot 4! \equiv 5 \cdot 6 \equiv 30 \equiv 3 \pmod 9$.
  \item So we want $(1 + 2 + 6 + 6 + 3) \bmod 9$.
  \item $=(9+9) \equiv 0 \pmod 9$.
\end{itemize}
\end{frame}


\begin{frame}{Example: Fast exponentiation by repeated squaring}
\begin{itemize}
  \item Compute $130^{90} \bmod 127$.
  \item Step 1. $130 \equiv 3 \pmod {127}$
  \item Reduce to $3^{90} \bmod 127$.
  \item Step 2. Start squaring and reducing mod 127.
  \item $3^2 = 9$.
  \item $3^4 = (3^2)^2 = 81$.
  \item $3^{8} = (3^4)^2 = 81^2 = 6561   \equiv 84  \pmod {127}$.
  \item $3^{16} = (3^{8})^2 \equiv 84^2  \equiv 71  \pmod {127}$.
  \item $3^{32} = (3^{16})^2 \equiv 71^2 \equiv 88  \pmod {127}$.
  \item $3^{64} = (3^{32})^2 \equiv 88^2 \equiv 124 \pmod {127}$.
\end{itemize}
\end{frame}

\begin{frame}{Example: Fast exponentiation by repeated squaring}
\begin{itemize}
  \item Step 3. Express 90 as a sum of powers of 2.
  \item $90 = 64+16+8+2$.
  \item Step 4. Plug in the values computed above.
  \item $3^{90} = 3^{64+16+8+2} = 3^{64} \cdot 3^{16} \cdot 3^{8} \cdot 3^{2}$
  \item $\equiv 124 \cdot 71 \cdot 84 \cdot 9  \pmod {127}$
  \item Step 5. Compute that product, incrementally reducing mod 127.
  \item $124 \cdot 71 \bmod 127 = 41$.
  \item $41 \cdot 84 \bmod 127 = 15$.
  \item $15 \cdot 9 \bmod 127 = 8$.
  \item So $130^{90} \bmod 127 = 8$.
\end{itemize}
\end{frame}





\end{document}
