\documentclass[oneside,12pt]{amsart}

\usepackage{amsmath,amssymb,latexsym,eucal,amsthm}

\input{mathdefs}
\input{theoremstyles}

\pagestyle{plain}

\begin{document}

\title{Homework Solutions \\ Math 310, Elementary Number Theory \\ Fall 2019}
\author{Mitch Rudominer}

\maketitle

\textbf{Solution to Exercise 2.3} Suppose $a+b = c$. We need to show that $a=c-b$.
By Axiom (4) $b$ has a unique additive inverse $-b$. Adding $-b$
to both sides of the equation, and
using axioms (1), (2) and (3) we get
$a= a+0 = a + (b + (-b)) = (a+b) + (-b) = c + (-b) = c-b$.

Now suppose that $a-b = c$. We want to show that $a=b+c$.
Adding $b$ to both sides of the equation and using
the axioms we get
$a = a + 0 = a + (-b + b) = (a - b) +b  = c + b = b+c$.

\bigskip


\textbf{Solution to Exercise 2.4} Fix integers $n,m$ and suppose that $n+m=n$.
We want to show that this implies that $m=0$.
By the previous exercise we  can subtract $n$ from both sides of the equation
to yield $m = n - n = 0$.


\bigskip


\textbf{Solution to Exercise 2.5} Fix integers $n,m$ and suppose that $n+m=0$.
We want to show that this implies that $n=-m$ and $m=-n$.
By Exercise 2.3 we can subtract $m$ from both sides of the equation to yield
 $n = 0+ (-m) = -m$ . Similarly we can subtract $n$ from both sides of the
 equation to yield $m=0+(-n) = -n$.

\bigskip


\textbf{Solution to Exercise 2.6} Since $0+0 = 0$, by the previous exercise
$0=-0$.


\bigskip


\textbf{Solution to Exercise 2.7} Since $(-n) + n = 0$, by exercise 2.5,
$-(-n) = n$.

\bigskip


\textbf{Solution to Exercise 2.9} Let $m=n\times 0$. To see that $m=0$, by
Excercise 2.4 it is enough to show that $n+m=n$.
$n+m = n + n\times 0 = n\times 1 + n\times 0
= n (1 + 0) = n \times 1 = n$.


\bigskip


\textbf{Solution to Exercise 2.13} Fix integers integers $a, b$.
We want to show that $(-a)b = a(-b) = -(ab)$. Using Lemma 2.12
we see that all three of these expressions are equal to $-1(ab)$.
$(-a)b=(-1\cdot a)b = -1(ab)$, $a(-b)=a(-1\cdot b) = -1(ab)$,
$-(ab) = -1(ab)$.


\bigskip


\textbf{Solution to Exercise 2.14} Let $m=n-1$. We need to show tht $m$ is
the predecessor of $n$. This means that $m<n$ and no integer lies between
$m$ and $n$. But this is true because $n=m+1$ so $n$ is the successor of $m$.


\bigskip


\textbf{Solution to Exercise 2.16} We are asked to show that $1$ is the least
positive integer. This is true because $1=0+1$ so $1$ is the successor of 0,
meaning $0 < 1$ and there is no integer between 0 and 1. But this means
that 1 is positive and there is no positive integer less than 1.

\bigskip


\textbf{Solution to Exercise 2.18} Let $S$ be the set of all positive real
numbers. This set does not have a minimal element.


\bigskip


\textbf{Solution to Exercise 2.20} We are asked to show that Axiom (2) follows
from Lemma 2.19. So assume that Lemma 2.19 is true and we will prove
Axiom (2). Let $n$ be negative. We need to show that $-n$ is positive.
By Lemma 2.19 we can add $-n$ to both sides of the inequality $n < 0$ to get
$n-n < 0 -n$ or $0 < -n$. So $-n$ is positive.

\bigskip


\textbf{Solution to Exercise 2.21} Suppose $n$ is positive. We will show $-n$
is negative. By Lemma 2.19 we can add $-n$ to both sides of the
ineqality $0<n$ to get $-n < n-n = 0$, so $-n$ is negative.


\bigskip


\textbf{Solution to Exercise 2.24} This exercise was not in the right place.
It is more natural for this exercise to come after Exercise 2.29 because we
want to use Exercises 2.28 and 2.29 in the proof. Fix integers $a,b$.
We need to show that $\av{ab} = \av{a}\av{b}$. We consider several cases.
If $a=0$ or $b=0$ then both sides of the equation
$\av{ab} = \av{a}\av{b}$ equal zero. If $a>0$ and $b>0$ then both sides of
the equation $\av{ab} = \av{a}\av{b}$ equal $ab$. If $a$ is positive and
$b$ negative then, then by Exercise 2.29, $ab$ is negative and so
$\av{ab} = -(ab) = a (-b) = \av{a}\av{b}$. The proof is similar if
$a$ is negative and $b$ is positive.

\bigskip


\textbf{Solution to Exercise 2.28} We are asked to show that the product of two
positive integers is positive. But this follows immediately from
Lemma  2.27 because if $a,b>0$ then $ab\geq a > 0$.

\bigskip


\textbf{Solution to Exercise 2.29} We need to prove that the product of a
positive integer and a  negative integer is negative. Suppose that $a>0$
and $b<0$. Then $-b>0$. By the previous exercise $a(-b) > 0$ and so
$ab = -(a(-b)) < 0$.

Now we need to prove that the product of two negative integers is positive.
Suppose that $a,b<0$. Then $-a,-b > 0$ so $ab = 1\cdot ab = -1\cdot-1\cdot ab
=-a\cdot-b$ is positive.

\bigskip


\textbf{Solution to Exercise 2.32} Let $a<b$ and $x>0$. We need to show
that $ax < bx$. By Lemma 2.25, $b-a$ is positive.
Since $x$ is also positive, we have $bx - ax = (b-a)x$,
which is the product of two positives and so is
positive. Thus by Lemma 2.24 again $ax < bx$.

Now, let $a<b$ and $x<0$. We need to show that $bx < ax$. By Lemma 2.25,
$b-a$ is positive. Since $x$ is negative we have $bx - ax = (b-a)x$, which
is the product of a positive and a negative and so is negative. Thus
$-(bx - ax) = (ax -bx)$ is positive. So $ax < bx$.

\bigskip


\textbf{Solution to Exercise 2.33} Fix integers $n$ and $m$ with $n\not=0$.
Suppose $n\times m=n$. We need to show that $m=1$. This follows from
the Cancellation Law, Lemma 2.31. Since $m\times n = 1 \times n$ and $n\not=0$,
we can cancel $n$ to get $m=1$.

\bigskip


\textbf{Solution to Exercise 3.4}

\textbf{(a)} We are asked to show that
$a\divides b$ iff $-a\divides b$ iff $a\divides -b$. This follows from the
fact that $b=ac$ iff $b = (-a)(-c)$ iff $-b = a(-c)$.

\bigskip

\textbf{(b)}Suppse  $a\divides b \And a\divides c$. We must show that
$a\divides (b+c)$. Let $d$ and $e$ be such that $b=ad$ and $c=ae$.
Let $f=d+e$.
Then $b+c = ad + ae = a(d+e) =af$. So $a\divides (b+c)$.

\bigskip

\textbf{(c)} Suppose $a\divides b \And b\divides c$. We must show that
$a\divides c$. Let $d$ and $e$ be such that
$b=ad$ and $c=be$. Let f = $de$. Then $c=be=ade = af$. So $a\divides c$.

\bigskip

\textbf{Solution to Exercise 3.14}
\begin{itemize}
\item $17 \mod 100 = 17$
\item $100 \mod 17 = 15$
\item $-17 \bmod 100 = 83$
\item $-100 \bmod 17 = 2$
\item $27 \bmod 3 = 0$
\item $4 \bmod 3 = 1$
\item $3 \bmod 3 = 0$
\item $2 \bmod 3 = 2$
\item $1 \bmod 3 = 1$
\item $0 \bmod  = 0$
\item $-1 \bmod 3 = 2$
\item $-2 \bmod 3 = 1$
\item $-3 \bmod 3 = 0$
\item $-4 \bmod 3 = 2$
\end{itemize}

\bigskip

\textbf{Solution to Exercise 1.1 on page 4 of \emph{Shoup}}.
Let $a,b,d\in\Z$ with $d\not=0$. Show that $a\divides b$ if and only if
$da\divides db$.
\begin{proof}
Suppose $a\divides b$ and let $c$ be such that $b=ac$. Then $bd=adc$ so
$ad \divides bd$. Conversely suppose $ad \divides bd$ and let $c$ be
such that $bd = adc$. Since $d\not=0$ we can cancel it to yield
$b=ac$. So $a\divides b$.
\end{proof}

\end{document}

