\documentclass[oneside,12pt]{amsart}

\usepackage{amsmath,amssymb,latexsym,eucal,amsthm}

\input{mathdefs}
\input{theoremstyles}

\pagestyle{plain}

\begin{document}

\title{Homework Solutions, Week 1 \\ Math 310, Elementary Number Theory \\ Fall 2019}
\author{Mitch Rudominer}

\maketitle

\textbf{Solution to Exercise 2.3} Suppose $a+b = c$. We need to show that $a=c-b$.
By Axiom (4) $b$ has a unique additive inverse $-b$. Adding $-b$
to both sides of the equation, and
using axioms (1), (2) and (3) we get
$a= a+0 = a + (b + (-b)) = (a+b) + (-b) = c + (-b) = c-b$.

Now suppose that $a-b = c$. We want to show that $a=b+c$.
Adding $b$ to both sides of the equation and using
the axioms we get
$a = a + 0 = a + (-b + b) = (a - b) +b  = c + b = b+c$.

\bigskip


\textbf{Solution to Exercise 2.4} Fix integers $n,m$ and suppose that $n+m=n$.
We want to show that this implies that $m=0$.
By the previous exercise we  can subtract $n$ from both sides of the equation
to yield $m = n - n = 0$.


\bigskip


\textbf{Solution to Exercise 2.5} Fix integers $n,m$ and suppose that $n+m=0$.
We want to show that this implies that $n=-m$ and $m=-n$.
By Exercise 2.3 we can subtract $m$ from both sides of the equation to yield
 $n = 0+ (-m) = -m$ . Similarly we can subtract $n$ from both sides of the
 equation to yield $m=0+(-n) = -n$.

\bigskip


\textbf{Solution to Exercise 2.6} Since $0+0 = 0$, by the previous exercise
$0=-0$.


\bigskip


\textbf{Solution to Exercise 2.7} Since $(-n) + n = 0$, by exercise 2.5,
$-(-n) = n$.

\bigskip


\textbf{Solution to Exercise 2.9} Let $m=n\times 0$. To see that $m=0$, by
Excercise 2.4 it is enough to show that $n+m=n$.
$n+m = n + n\times 0 = n\times 1 + n\times 0
= n (1 + 0) = n \times 1 = n$.


\bigskip


\textbf{Solution to Exercise 2.13} Fix integers integers $a, b$.
We want to show that $(-a)b = a(-b) = -(ab)$. Using Lemma 2.12
we see that all three of these expressions are equal to $-1(ab)$.
$(-a)b=(-1\cdot a)b = -1(ab)$, $a(-b)=a(-1\cdot b) = -1(ab)$,
$-(ab) = -1(ab)$.

\end{document}

